# The First-Order Linear Recurrence Relation

## Definition of Recurrence Relation

A recurrence relation is an equation that defines the relationship between the $n$-th term of a sequence and its proceeding terms within the sequence. It expresses how each term depends on one or more proceeding terms in sequence.

## Difference Operator

Difference operator: $\Delta$

### First Order

- **first order:**
$\Delta a_n = a_{n+1} - a_n$
- **second order:**
$\begin{aligned}
\Delta^2 a_n &= \Delta a_{n+1} - \Delta a_n \\
&= (a_{n+2} - a_{n+1}) - (a_{n+1} - a_n) \\ 
&= a_{n+2} - 2a_{n+1} + a_n
\end{aligned}$
- **third order:**
$\begin{aligned}
\Delta^3 a_n &= \Delta^2 a_{n+1} - \Delta^2 a_n \\
&= (a_{n+1} -2a_{n+2} + an_{n+1}) - (a_{n+2} - 2a_{n+1} + a_n) \\
&= a_{n+3} - 3a_{n+2} + 3 a_{n+1} - a_n
\end{aligned}$

### Example

$$\begin{aligned}
a_n &= n^3 - 2n^2 + 3n - 2 \\
\Delta a_n &= (n+1)^3 - 2(n+1)^2 + 3 (n+1) - 2 - (n^3 - 2n^2 + 3n - 2) \\
&= 3n^2 - n + 2 \\
\Delta^2 a_n &= \Delta a_{n+1} - \Delta a_n \\
&= 3(n+1)^2 - (n+1) + 2 - (3n^2 - n + 2) \\
&= 6n + 2 \\
\Delta^3 a_n &= \Delta^2 a_{n+1} - \Delta^2 a_n \\
&= 6(n+1) + 2 - (6n + 2) \\
&= 6
\end{aligned}$$

## Difference equation and recurrence relation

$$\begin{aligned}
&\Delta^2 a_n + \Delta a_n - a_n = 0 \\
&\Harr (a_{n+2} - 2a_{n+1} + a_n) + (a_{n+1} - a_n) - a_n = 0 \\
&\Harr a_{n+2} = a_{n+1} + a_n
\end{aligned}$$

## Definition of k-th order linear recurrence relation

Consider a sequence $a_n$. A $k$th order linear recurrence relation with constant coefficient is an equation of the form :
$$\sum_{i=0}^{k}c_{n-k}a_{n-k} = f(n)$$
where $n \geq k$, $c_n$ are known constants with $c_n \neq 0$, and $c_{n-k} \neq 0$. The function $f(n)$ represents any given function of $n$.

This relation describes how each term of the sequence $a_n$ is related to the $k$ preceding terms in the sequence, weighted by the constants $c_n$.

## Definition of first-order recurrence relation

A first-order linear recurrence relation is a mathematical formula that describe the relation between a successive terms in sequence. It could  be represented in the form:
$$a_{n+1} = c * a_n + d$$
where $a_n$ is the $n$th term in the sequence, $a_{n+1}$ is the next term, $c$ and $d$ a constant, and $n$ is a non-negative integer.

## Characteristic

- **Linear:** The relation between successive terms is linear, meaning each term is constant multiple of the previous term plus another constant.
- **First-order:** The relation involves only one previous term to determine the next term.

## Relation

Define a recurrence relation in the form:
$$a_n = 3a_n, \space n \geq 0, \space a_0 = 5$$

The first four terms of this sequence are calculated as follows:
$$\begin{aligned}
a_0 &= 5 \\
a_1 &= 3a_0 &&=3(5) \\
a_2 &= 3a_1 &&= 3(3a_0) &&&= 3^2(5) \\
a_3 &= 3a_2 &&= 3(3^2(5)) &&&= 3^3(5)
\end{aligned}$$

## Unique Solution

From the relation above, we can observe a pattern in the terms of the sequence:
$$a_n = 5 * 3^n, \space n \geq 0$$
This pattern suggests that the unique solution to the recurrence relation of the form $a_{n+1} = ca_n$, where $c$ is a constant and $a_0 = A$ is given by:
$$a_n = A * d^n, \space n \geq 0$$
In our case, $A=5$ and $d=3$, so the solution is:
$$a_n = 5 * 3^n, \space n \geq 0$$