# Second-Order Linear Homogeneous Recurrence Relation

## Worm up

Let $S = \{ 1, 2, 3, ..., n \}$.
Define $a_n$ as the number of the subsets of $S$ that contain no consecutive integers.
Find the unique solution of $a_n$

### Solution

Let $A$ be any subsets of $S$ that contains no consecutive integers. TO find the unique solution for $a_n$, consider the following possibilities:

1. If $n \in A$, then $(n-1) \notin A$, and the subset $A - \{ n \}$ will be counted in $a_{n-2}$ because removing $n$ from $A$ ensures that there are no consecutive integers in the subset.
2. If $n \notin A$, then the subset $A$ will be counted in $a_{n-1}$ because $n$ can be added to any subset $A$ that contains no consecutive integers to form a valid subset of $S$.

Therefore, the unique solution for $a_n$ is given by the recurrence relation :
$$ a_n = a_{n-1} + a_{n-2}$$

---

Let $k \in \mathcal{Z}^+$ and $C_0, C_1, C_2, ..., C_k$ is a real number sequence.
If $a_n$, for $n \geq 0$, is a discrete function, then:
$$C_0a_n + C_1a_{n-1} + C_2a_{n-2} + ... + C_ka_{n-k} = f(n)$$

## Homogeneous

If $C_0a_n + C_1a_{n-1} + C_2a_{n-2} + ... + C_ka_{n-k} = 0$, it is called **homogeneous**; otherwise, it is called **nonhomogeneous**.

## Characteristic Equation

Substituting $a_n = cr^n$ into $C_0a_n + C_1a_{n-1} + C_2a_{n-2}$, we obtain:
$$C_0cr^n + C_1cr^{n-1} + C_2cr^{n-2} = 0$$

With $c, r \neq 0$, it becomes $C_0r^2 + C_1r + C_2 = 0$. The quadratic equation of this function is called **characteristic equation**.

Regardless of whether the roots $r_1$ and $r_2$ are distinct real numbers, identical real numbers, or a complex conjugate pair, they are referred as **characteristic roots** of the recurrence relation.

---

## Solution for Distinct Real Roots

To solve a recurrence relation: $Aa_n + B_{n-1} + Ca_{n-2} = 0$, where $n \geq 2$ and $a_0 = x_1, a_1 = x_2$

Let $a_n = cr^n$, we get $Acr^n + Bcr^{n-1} + Ccr^{n-2} = 0$, and the characteristic equation is $Ar^2 + Br + C = 0$, where the root is $r_1$ and $r_2$.

We write $a_n = c_1 (r_1)^n + c_2 (r_2)^n$ as a **general solution**.
Finally, use the known condition, like $a_0 = x_1, \space a_1 = x_2$, to solve $c_1$ and $c_2$.

---

### Example

Solve the recurrence relation $a_n + a_{n-1} - 6a_{n-2} = 0$, where $n \geq 2$ and $a_0 = -1, \space a_1 = 8$.

If $a_n = cr^n$, we obtain $cr^n + cr^{n-1} - 6cr^{n-2} = 0$ from which the characteristic equation $r^2 + r - 6 = 0$ follow:
$$ 0 = r^2 + r - 6 = (r+3)(r-2) \Rightarrow r = 2, \space -3$$

Since we have two distinct roots, $a_n = (2)^n$ and $a_n = (-3)^n$ are both solutions of this sequence.
They are **linearly independent** solution because one is not a multiple of the other; that is, there is no real constant $k$ such that $(-3)^n = k(2)^n$ for *all* $n \in \mathcal{N}^+$. And by the **first superposition principle**, we write $a_n = c_1(2)^n + c_2(-3)^n$.
With $a_0 = -1$ and $a_1 = 8$, $c_1$ and $c_2$ are determined as follows:
$$\begin{aligned}
-1 &= a_0 &&= c_1(2)^0 + c_2(-3)^0 &&= c_1 + c_2 \\
8 &= a_1 &&= c_1(2)^1 + c_2(-3)^1 &&= 2c_2 - 3c_2
\end{aligned}$$

Solving this system of equations, one find $c_1 = 1, c_2 = -2$. Therefore, $a_n = 2^n - 2(-3)^n, \space n \geq 0$, is the unique solution of the given recurrence relation.

---

## Lemma

if $f(x) = 0$ has multiple roots $a$ then $f^{'}(x) = 0$

### Example

$f(x) - x^2 - 2x +1$
$0 = x^2 - 2x +1, \space x = 1, 1$
$f^{'}(x) = 2x-2 \Rightarrow f^{'}(1) = 0$

## Solution for Repeated Roots

Consider a recurrence relation with characteristic roots $r_1, r_2$ which are the same real number, i.e., the roots are repeated.

Typically, if the roots were distinct, the solutions would simply be of the form $a_n = k * r^n$. However, when roots are repeated, as in this case, we come across additional solutions of the form $a_n = n*r^n$.

The full solution methods goes as follow:

1. Start with the original recurrence relation denote as:
$c_n r_1^n + c_{n-1} r_1^{n-1} + c_{n-2} r_1^{n-2} = 0$.
2. By lemma, identify that $r_1$ is also a root of the derivative of this equation, given by $c_n(n)r_1^{n-1} + c_{n-1}(n-1)r_1^{n-2} + c_{n-2}(n-2)r_1^{n-3} = 0$.
3. Multiply this derivative by $r_1$ to yield:
$c_n(n)r_1^n + c_{n-1}(n-1)r_1^{n-1} + c_{n-2}(n-2)r_1^{n-2} = 0$.

To observe the equation, we are essentially getting $nr_1^n$ instead of just $r_1^n$, indirectly proving that $a_n = nr_1^n$ is a valid solution to the recurrence relation when roots are repeated.

Thus our general solution becomes
$$\begin{aligned}
a_n &= k_1(r_1)^n + k_2n(r_1)^n \\
&= (k_1 + k_2n)(r_1)^n
\end{aligned}$$

### Example

Given the recurrence relation $a_n - 6a_{n-1} + 9a_{n-2} = 0$ with $a_0 = 5$ and $a_1 = 12$, find $a_n$.

Its characteristic equation, $r^2 - 6r + 9 = 0$, returns the root $r = 3$.
This guides us to the solution form $a_n = (k_1 + k_2n)(3)^n$.

Applying the initial values:

- For $n = 0$: $a_0 = k_1(3)^0 = 5$ gives $k_1 = 5$.
- For $n = 1$: $a_1 = (5 + k_2)(3)^1 = 12$ leads to $k_2 = -1$.

Then, our desired solution is $a_n = (5-n)(3)^n$.

---

## DeMoivre's Theorem

$$(\cos{\theta} + i\sin{\theta})^n = \cos{n\theta} + i\sin{n\theta}$$
$$z = x + yi = r(\cos{\theta} + i\sin{\theta}), \text{ where r = }\sqrt{x^2 + y^2}, \space \theta = \arctan{y/x}$$
in all cases:
$$z^n = (x + yi)^n = r^n(\cos{n\theta} + i\sin{n\theta})$$

## Solution for Complex Roots

Given the general solution $a_n = c_1(x = yi)^n + c_2(x - yi)^n$, where $(x + yi)$ and $(x - yi)$ are complex roots.

Let's express $(x + yi)$ and $(x - yi)$ in polar form:

- $r = \sqrt{x^2 + y^2}$
- $(x + yi) = r(\cos{\theta} + i\sin{\theta})$
- $(x - yi) = r(\cos{-\theta} + i\sin{-\theta}) = r(\cos{\theta} - i\sin{\theta})$

Substituting these expression into $a_n$, we get:
$a_n = c_1[r(\cos{\theta} + i\sin{\theta})]^n + c_2[r(\cos{\theta} - i\sin{\theta})]^n$

Simplifying the expression using DeMoivre's theorem, we have:
$a_n = c_1(r)^n(\cos{(n\theta)} + i\sin{(n\theta)}) + c_2(r)^n(\cos{(n\theta)} - i\sin{(n\theta)})$

Grouping real and imaginary parts together, we get:
$a_n = r^n(k_1 \cos{n\theta} + k_2 \sin{n\theta})$
where $k_1 = c_1 + c_2$ and $k_2 = (c_1 - c_2)i$

Lastly, the initial condition can be used to solve for $k_1$ and $k_2$.

---

### Example

Solve the recurrence relation $a_n = 2(a_{n-1} - a_{n-2})$, where $n \geq 2$ and $a_0 = 1$, $a_1 = 2$

Letting $a^n = cr^n$, for $c, r \neq 0$, we get $r^2 - 2r + 2 = 0$, whose roots are
<font color=#FF5151>EDIT</font>